\begin{center}
    \AXC{$[\ ]\ cont$}
    \RightLabel{Nat-I$_1$)}
    \UIC{$0 \in Nat\ [\ ]$}
    \noLine
    \UIC{(\textbf{Ax1})}
\DisplayProof
\hspace{.1in}
    \AXC{$[\ ]\ cont$}
    \RightLabel{Nat-F)}
    \UIC{$Nat\ type\ [\ ]$}
    \RightLabel{F-c)}
    \UIC{$x \in Nat\ cont$}
    \RightLabel{var)}
    \UIC{$x \in Nat\ [x \in Nat]$}
    \RightLabel{I-Id)}
    \UIC{$id(x) \in Id(Nat, x, x)\ [x \in Nat]$}
    \RightLabel{I-$\to$)}
    \UIC{$ \lambda x. id(x) \in \Pi_{x \in Nat} Id(Nat, x, x)\ [\ ]$}
    \noLine
    \UIC{(\textbf{Ax2})}
\DisplayProof
\end{center}

\begin{prooftree}
    \AXC{(Simmetry \ref{es:simmetry})}
    \RightLabel{E-Id)}
    \UIC{$El_{Id} (w, id) \in Id(Nat, y, x)\ [x \in Nat, y \in Nat, w \in  Id(Nat, x, y)]$}
    \RightLabel{I-$\to$)}
    \UIC{$\lambda w. El_{Id} (w, id) \in Id(Nat, x, y) \rightarrow Id(Nat, y, x)\ [x \in Nat, y \in Nat]$}
    \RightLabel{I-$\Pi$)}
    \UIC{$\lambda y. \lambda w. El_{Id} (w, id) \in \Pi_{y \in Nat} Id(Nat, x, y) \rightarrow Id(Nat, y, x)\ [x \in Nat]$}
    \RightLabel{I-$\Pi$)}
    \UIC{$\lambda x. \lambda y. \lambda w. El_{Id} (w, id) \in \Pi_{x \in Nat} \Pi_{y \in Nat} Id(Nat, x, y) \rightarrow Id(Nat, y, x)\ [\ ]$}
    \noLine
    \UIC{(\textbf{Ax3})}
\end{prooftree}
\begin{prooftree}
    \AXC{(Transitivity, Martin-Löf’s \ref{es:transitivity_ml})}
    \RightLabel{E-$\to$)}
    \UIC{$Ap(El_{Id}(w_2,\lambda w.w),w_1)\in Id(Nat, x, z)\ [x \in Nat, y \in Nat, z \in Nat, w_1 \in Id(Nat, x, y), w_2 \in Id(Nat, y, z)]$}
    \RightLabel{I-$\Pi$)}
    \UIC{$\lambda w_2. Ap(El_{Id}(w_2,\lambda w.w),w_1)\in Id(Nat, y, z) \rightarrow Id(Nat, x, z)\ [\Gamma, w_1 \in Id(Nat, x, y)]$}
    \RightLabel{I-$\Pi$)}
    \UIC{$\lambda w_1. \lambda w_2. Ap(El_{Id}(w_2,\lambda w.w),w_1)\in Id(Nat, x, y) \rightarrow Id(Nat, y, z) \rightarrow Id(Nat, x, z)\ [\Gamma, z \in Nat]$}
    \RightLabel{I-$\Pi$)}
    \UIC{$\lambda z. \lambda w_1. \lambda w_2. Ap(El_{Id}(w_2,\lambda w.w),w_1)\in \Pi_{z \in Nat} Id(Nat, x, y) \rightarrow Id(Nat, y, z) \rightarrow Id(Nat, x, z)\ [\Gamma, y \in Nat]$}
    \RightLabel{I-$\Pi$)}
    \UIC{$\lambda y. \lambda z. \lambda w_1. \lambda w_2. Ap(El_{Id}(\cdots),w_1)\in \Pi_{y \in Nat} \Pi_{z \in Nat} Id(Nat, x, y) \rightarrow Id(Nat, y, z) \rightarrow Id(Nat, x, z)\ [x \in Nat]$}
    \RightLabel{I-$\Pi$)}
    \UIC{$\lambda x. \lambda y. \lambda z. \lambda w_1. \lambda w_2. Ap(El_{Id}(\cdots),w_1)\in \Pi_{x \in Nat} \Pi_{y \in Nat} \Pi_{z \in Nat} Id(Nat, x, y) \rightarrow Id(Nat, y, z) \rightarrow Id(Nat, x, z)\ [\ ]$}
    \noLine
    \UIC{(\textbf{Ax4})}
\end{prooftree}


\begin{prooftree}
    \AXC{$[\ ]\ cont$}
    \UIC{$\vdots$}
    \noLine
    \UIC{$a \in Nat\ [a \in Nat, w \in Id(Nat, a, b)]$}
    \AXC{(1)}
    \noLine
    \UIC{$a = b \in Nat\ [a \in Nat, w \in Id(Nat, a, b)]$}
    % \RightLabel{)}
    \BIC{$b \in Nat\ [a \in Nat, w \in Id(Nat, a, b)]$}
    \noLine
    \UIC{(\textbf{Ax5})}
\end{prooftree}
\begin{center}
    $(1)\qquad$sse $nf(a) \equiv nf(b)$ allora con la prova $w$ posso concludere con l'uguaglianza computazionale
\end{center}
\begin{prooftree}
    \AXC{$[\ ]\ cont$}
    \RightLabel{Nat-F)}
    \UIC{$Nat\ type\ [\ ]$}
    \RightLabel{F-c)}
    \UIC{$x \in Nat\ cont$}
    \RightLabel{var)}
    \UIC{$x \in Nat\ [x \in Nat]$}
    \RightLabel{Nat-I$_2$)}
    \UIC{$succ(x)\in Nat\ [x \in Nat]$}
    \noLine
    \UIC{(\textbf{Ax6})}
\end{prooftree}
\newpage

\begin{prooftree}
    \AXC{$[\ ]\ cont$}
    \UIC{$\vdots$}
    \noLine
    \UIC{$x' \in Nat\ [\Gamma]$}
    \AXC{$[\ ]\ cont$}
    \UIC{$\vdots$}
    \noLine
    \UIC{$0 \in Nat\ [\Gamma]$}
    \AXC{$[\ ]\ cont$}
    \UIC{$\vdots$}
    \noLine
    \UIC{$x \in Nat\ [\Gamma, x \in Nat, z \in Nat]$}
    \RightLabel{Nat-e)}
    \TIC{$El_{Nat}(x', 0, (x, z).x)\in Nat\ [\Gamma, x' \in Nat)]$}
    \dashedLine
    \UIC{$prec(x')\in Nat\ [\Gamma, x' \in Nat)]$}
    \RightLabel{I-Id)}
    \UIC{$id(prec(x'))\in Id(Nat, prec(x'), prec(x'))\ [\Gamma, x' \in Nat)]$}
    \noLine
    \UIC{(C)}
\end{prooftree}

\begin{prooftree}
    \AXC{$Id(Nat, prec(\hat{x}), prec(\hat{y}))\ type\ [\Gamma, \hat{x} \in Nat, \hat{y} \in Nat, z \in Id(Nat, \hat{x}, \hat{y})]$}
    \noLine
    \UIC{(B)}
\end{prooftree}

\begin{prooftree}
    \AXC{(B)}
    \noLine
    \UIC{$\cdots$}
    \AXC{$succ(x) \in Nat\ [\Gamma]$}
    \AXC{$succ(y) \in Nat\ [\Gamma]$}
    \AXC{$b \in Id(Nat, succ(x), succ(y))$}
    \AXC{(C)}
    \noLine
    \UIC{$\cdots$}
    \RightLabel{E-Id)}
    \QuinaryInfC{$El_{Id} (b, (x').id(prec(x'))) \in Id(Nat, prec(succ(x)), prec(succ(y)))\ [\Gamma, b \in Id(Nat, succ(x), succ(y))]$}
    \dashedLine
    \RightLabel{(2)}
    \UIC{$El_{Id} (b, (x').id(prec(x'))) \in Id(Nat, x, y)\ [\Gamma, b \in Id(Nat, succ(x), succ(y))]$}
    \RightLabel{I-$\to$)}
    \UIC{$\lambda b.El_{Id} (b, (x').id(prec(x'))) \in Id(Nat, succ(x), succ(y)) \rightarrow Id(Nat, x, y)\ [\Gamma]$}
    \noLine
    \UIC{(A)}
\end{prooftree}

\begin{prooftree}
    \AXC{(Equality preservation among programs \ref{es:eq_preservation_programs})}
    \LeftLabel{E-Id)}
    \UIC{$El_{Id}(a, (z).id(succ(z))) \in Id(Nat, succ(x), succ(y))\ [\Gamma, a \in Id(Nat, x, y)]$}
    \LeftLabel{I-$\to$)}
    \UIC{$\lambda a.El_{Id}(a, (z).id(succ(z))) \in Id(Nat, x, y) \rightarrow Id(Nat, succ(x), succ(y))\ [\Gamma]$}
    \AXC{(A)}
    \noLine
    \UIC{$\cdots$}
    % \AXC{$\lambda b.\cdots \in Id(Nat, succ(x), succ(y)) \rightarrow Id(Nat, x, y)\ [\Gamma]$}
    \LeftLabel{I-$\times$)}
    \BIC{$\langle \lambda a.\cdots, \lambda b.\cdots\rangle\in Id(Nat, x, y) \leftrightarrow Id(Nat, succ(x), succ(y))\ [x \in Nat, y \in Nat]$}
    \RightLabel{I-$\Pi$)}
    \UIC{$\lambda y. \langle \lambda a.\cdots, \lambda b.\cdots\rangle\in \Pi_{y \in Nat} Id(Nat, x, y) \leftrightarrow Id(Nat, succ(x), succ(y))\ [x \in Nat]$}
    \RightLabel{I-$\Pi$)}
    \UIC{$\lambda x. \lambda y. \langle \lambda a.\cdots, \lambda b.\cdots\rangle\in \Pi_{x \in Nat} \Pi_{y \in Nat} Id(Nat, x, y) \leftrightarrow Id(Nat, succ(x), succ(y))\ [\ ]$}
    \noLine
    \UIC{(\textbf{Ax7})}
\end{prooftree}

\begin{align*}
    (2)\qquad prec\quad\equiv\quad &El_{Nat}(x, 0, (x, z).x) \in Nat\ [x \in Nat] \ Dove:\\
    &El_{Nat} (succ(x), 0, (x, z).x) = x \in Nat\ [x \in Nat]\\
    &El_{Nat} (0, 0, (x, z).x) = 0 \in Nat\ [x \in Nat]
\end{align*}

\begin{prooftree}
    \AXC{(Nat terms inequality \ref{es:nat_inequality})}
    \RightLabel{I-$\to$)}
    \UIC{$\lambda w. Ap(\pi_1(k(\hat{N_1}, \hat{N_2}, p_f(w))), \star)\in Id(Nat, 0, succ(x)) \rightarrow N_0\ [x \in Nat]$}
    \RightLabel{I-$\Pi$)}
    \UIC{$\lambda x. \lambda w. Ap(\pi_1(k(\hat{N_1}, \hat{N_2}, p_f(w))), \star)\in \Pi_{x \in Nat} Id(Nat, 0, succ(x)) \rightarrow N_0\ [\ ]$}
    \noLine
    \UIC{(\textbf{Ax8})}
\end{prooftree}

\begin{prooftree}
    \AXC{$\pi_1$}
    \noLine
    \UIC{$D\ type\ [\Gamma]$}
    \AXC{$[\ ]\ cont$}
    \RightLabel{Nat-F)}
    \UIC{$Nat\ type\ [\ ]$}
    \RightLabel{var)}
    \UIC{$x \in Nat\ [x \in Nat]$}
    \AXC{$\pi_2$}
    \noLine
    \UIC{$0 \in D\ [\Gamma]$}
    \AXC{$\pi_3$}
    \noLine
    \UIC{$succ(x') \in D\ [x \in Nat, x' \in Nat, z \in Nat]$}
    \RightLabel{Nat-e)}
    \QuaternaryInfC{$El_{Nat}(x, 0, (x', z).succ(x')) \in D\ [x \in Nat]$}
    \noLine
    \UIC{(\textbf{Ax9})}
\end{prooftree}